WIP

src/specs/EvaluateLagrangePolyOutOfDomain.ec
@@ -39,49 +39,51 @@ module EvaluateLagrangePolyOutOfDomain = {
     return ret;
   }
 
-  proc low'(polyNum: uint256, at: uint256): uint256 = {
-  var ret, omegaPower, tmp267, _10, denominator;
-    tmp267 <@ Modexp.low(at, (W256.of_int Constants.DOMAIN_SIZE));
+  (* proc low'(polyNum: uint256, at: uint256): uint256 = { *)
+  (* var ret, omegaPower, tmp267, _10, denominator; *)
+  (*   tmp267 <@ Modexp.low(at, (W256.of_int Constants.DOMAIN_SIZE)); *)
 
-    omegaPower <- (W256.of_int 1);
-    if ((bool_of_uint256 polyNum))
-    {
-      omegaPower <@ Modexp.low((W256.of_int Constants.OMEGA), polyNum);
-    }
+  (*   omegaPower <- (W256.of_int 1); *)
+  (*   if ((bool_of_uint256 polyNum)) *)
+  (*   { *)
+  (*     omegaPower <@ Modexp.low((W256.of_int Constants.OMEGA), polyNum); *)
+  (*   } *)
     
-    ret <- (PurePrimops.addmod tmp267 ((W256.of_int Constants.R) - W256.one) (W256.of_int Constants.R));
-    if ((bool_of_uint256 (PurePrimops.iszero ret)))
-    {
-      RevertWithMessage.low(W256.of_int 28, W256.of_int STRING);
-    }
+  (*   ret <- (PurePrimops.addmod tmp267 ((W256.of_int Constants.R) - W256.one) (W256.of_int Constants.R)); *)
+  (*   if ((bool_of_uint256 (PurePrimops.iszero ret))) *)
+  (*   { *)
+  (*     RevertWithMessage.low(W256.of_int 28, W256.of_int STRING); *)
+  (*   } *)
     
-    ret <- (PurePrimops.mulmod ret omegaPower (W256.of_int Constants.R));
-    _10 <- ((W256.of_int Constants.R) - omegaPower);
-    denominator <- (PurePrimops.addmod at _10 (W256.of_int Constants.R));
-    denominator <- (PurePrimops.mulmod denominator (W256.of_int Constants.DOMAIN_SIZE) (W256.of_int Constants.R));
-    denominator <@ Modexp.low(denominator, ((W256.of_int Constants.R) - (W256.of_int 2)));
-    ret <- (PurePrimops.mulmod ret denominator (W256.of_int Constants.R));
-    return ret;
-  }
+  (*   ret <- (PurePrimops.mulmod ret omegaPower (W256.of_int Constants.R)); *)
+  (*   _10 <- ((W256.of_int Constants.R) - omegaPower); *)
+  (*   denominator <- (PurePrimops.addmod at _10 (W256.of_int Constants.R)); *)
+  (*   denominator <- (PurePrimops.mulmod denominator (W256.of_int Constants.DOMAIN_SIZE) (W256.of_int Constants.R)); *)
+  (*   denominator <@ Modexp.low(denominator, ((W256.of_int Constants.R) - (W256.of_int 2))); *)
+  (*   ret <- (PurePrimops.mulmod ret denominator (W256.of_int Constants.R)); *)
+  (*   return ret; *)
+  (* } *)
   
   proc mid(polyNum: int, at: int): int option = {
-    var r, omegaP, zd1, num, den, inv;
+    var r, omegaPolyNum, atDomainSize, zd1, num, den, inv;
 
-    omegaP <@ Modexp.mid(OMEGA, polyNum);
-    zd1 <- (at^DOMAIN_SIZE - 1) %% R;
+    omegaPolyNum <- (OMEGA ^ polyNum) %% R; 
+    atDomainSize <- (at ^ DOMAIN_SIZE) %% R; 
+    
+    zd1 <- (atDomainSize - 1) %% R;
     
     if(zd1 = 0) {
       r <- None;
     } else {
-      num <- (omegaP * zd1) %% R;
-      den <- (DOMAIN_SIZE * (at - omegaP)) %% R;
+      num <- (omegaPolyNum * zd1) %% R;
+      den <- (DOMAIN_SIZE * (at - omegaPolyNum)) %% R;
       inv <- den^(R - 2) %% R;
       r <- Some ((num * inv) %% R);
     }  
     return r;
   }
 }.
-
+    
 lemma evaluateLagrangePolyOutOfDomain_extracted_equiv_low:
     equiv [
       Verifier_1261.usr_evaluateLagrangePolyOutOfDomain ~ EvaluateLagrangePolyOutOfDomain.low :
@@ -118,7 +120,28 @@ lemma evaluateLagrangePolyOutOfDomain_extracted_equiv_low:
         sp. skip. by progress.
     qed.
 
-lemma evaluateLagrangePolyOutOfDomain_low_equiv_mid (memory : mem) (poly256 at256 r: uint256):
+lemma modexp_same (m: mem) (v1 v2 p1 p2 r1 r2 : uint256) : 
+    modexp_memory_footprint (modexp_memory_footprint m v1 p1 r1) v2 p2 r2 =
+    modexp_memory_footprint m v2 p2 r2.
+proof. admit. qed.
+
+lemma modexp_pspec (m : mem) (base power : uint256) :
+    phoare [ Modexp.low :
+      arg = (base, power) /\
+      Primops.memory = m /\
+      !Primops.reverted
+      ==>
+      !Primops.reverted /\
+      Primops.memory = modexp_memory_footprint m base power res /\
+      res = W256.of_int (((W256.to_uint base) ^ (W256.to_uint power)) %% R)
+    ] = 1%r.
+proof. admit. qed.
+
+lemma modexp_low_pspec_revert :
+phoare [ Modexp.low : Primops.reverted ==> Primops.reverted ] = 1%r.
+proof. proc; inline*; wp; by progress. qed.
+
+lemma evaluateLagrangePolyOutOfDomain_low_equiv_mid (memory : mem) (poly256 at256: uint256):
 equiv [
     EvaluateLagrangePolyOutOfDomain.low ~ EvaluateLagrangePolyOutOfDomain.mid :
       arg{1} = (poly256, at256) /\
@@ -128,6 +151,7 @@ equiv [
       ==>
       (
         !Primops.reverted{1} /\
+        ((W256.to_uint at256)^DOMAIN_SIZE - 1) %% Constants.R <> 0 /\
         res{2} = Some (to_uint res{1})%W256)
       \/
       (
@@ -137,12 +161,152 @@ equiv [
       )
     ].
 proof. proc.
-seq 2 1 : (#pre /\ omegaPower{1} = W256.of_int omegaP{2}).
-seq 1 0 : (#pre /\ omegaPower{1} = W256.one). wp. skip. auto.
+    
+seq 2 1 : (
+  (polyNum{1}, at{1}) = (poly256, at256) /\
+  (polyNum{2}, at{2}) = (to_uint poly256, to_uint at256) /\
+  !Primops.reverted{1} /\
+  ((poly256 <> W256.zero /\ Primops.memory{1} = (modexp_memory_footprint memory (W256.of_int OMEGA) polyNum{1} omegaPower{1})) 
+  \/
+  (poly256 = W256.zero /\ Primops.memory{1} = memory)
+  )
+  /\
+  omegaPower{1} = W256.of_int omegaPolyNum{2} /\ omegaPolyNum{2} = (OMEGA ^ polyNum{2}) %% R
+). wp. sp. 
 case (bool_of_uint256 polyNum{1}).
+(* polyNum != 0 *)
 rcondt{1} 1. by progress.
-call (modexp_low_equiv_mid memory (W256.of_int OMEGA) poly256).
-skip. progress. smt. admit. (* HERE *)
+call{1} (modexp_pspec memory (W256.of_int OMEGA) poly256).
+skip. progress. left. by auto.
+rewrite !W256.of_uintK. have ->: OMEGA %% W256.modulus = OMEGA. by smt(). by reflexivity.
 rcondf{1} 1. by progress.
+skip. progress. right. by auto.
+have ->: polyNum{1} = W256.zero. by smt(). progress. by smt().
+
+seq 1 1: (
+  (polyNum{1}, at{1}) = (poly256, at256) /\
+  (polyNum{2}, at{2}) = (to_uint poly256, to_uint at256) /\
+  !Primops.reverted{1} /\
+  Primops.memory{1} = modexp_memory_footprint memory at{1} (W256.of_int DOMAIN_SIZE) tmp267{1} /\
+  omegaPower{1} = W256.of_int omegaPolyNum{2} /\ omegaPolyNum{2} = (OMEGA ^ polyNum{2}) %% R /\
+  tmp267{1} = W256.of_int atDomainSize{2} /\ atDomainSize{2} = (at{2} ^ DOMAIN_SIZE) %% R
+).
+wp. 
+exists* omegaPower{1}. elim* => oP.
+pose mem' := (modexp_memory_footprint memory ((of_int OMEGA))%W256 poly256 oP).
+case (poly256 = W256.zero).
+call{1} (modexp_pspec memory at256 (W256.of_int DOMAIN_SIZE)).
+skip. progress. by smt().
+rewrite !W256.of_uintK. have ->: DOMAIN_SIZE %% W256.modulus = DOMAIN_SIZE. by smt(). reflexivity.
+call{1} (modexp_pspec mem' at256 (W256.of_int DOMAIN_SIZE)).
+skip. progress. by smt(). apply modexp_same.
+rewrite !W256.of_uintK. have ->: DOMAIN_SIZE %% W256.modulus = DOMAIN_SIZE. by smt(). reflexivity.
+
+seq 1 1: (#pre /\ ret{1} = W256.of_int zd1{2} /\ zd1{2} = (atDomainSize{2} - 1) %% R).
+wp. skip. progress.
+rewrite /addmod. progress. rewrite !W256.of_uintK !mod_R_W256_mod_R !R_mod_W256_R.
+have ->: (R - 1) %% W256.modulus = R - 1. by smt(). by smt.
+
+if. progress.
+rewrite /bool_of_uint256 /iszero in H0.
+case ((of_int ((to_uint at{1} ^ DOMAIN_SIZE %% R - 1) %% R))%W256 = W256.zero).
+progress. by smt.
+progress. by smt.
+by smt.
+
+seq 1 1: ((to_uint at256 ^ DOMAIN_SIZE - 1) %% R = 0 /\ r{2} = None /\ Primops.reverted{1}).
+wp. call{1} revertWithMessage_low_pspec. skip. progress. by smt.
+wp. sp. call{1} modexp_low_pspec_revert. skip. progress.
+
+seq 1 1: (
+(polyNum{1}, at{1}) = (poly256, at256) /\
+(polyNum{2}, at{2}) = (to_uint poly256, to_uint at256) /\
+!Primops.reverted{1} /\
+Primops.memory{1} = modexp_memory_footprint memory at{1} ((of_int DOMAIN_SIZE))%W256 tmp267{1} /\
+omegaPower{1} = (of_int omegaPolyNum{2})%W256 /\ omegaPolyNum{2} = OMEGA ^ polyNum{2} %% R /\
+tmp267{1} = (of_int atDomainSize{2})%W256 /\ atDomainSize{2} = at{2} ^ DOMAIN_SIZE %% R /\
+ret{1} = (of_int num{2})%W256 /\ num{2} = (omegaPolyNum{2} * zd1{2}) %% R /\
+zd1{2} = (atDomainSize{2} - 1) %% R /\ zd1{2} <> 0
+).
+wp. skip. progress.
+rewrite /mulmod. progress. rewrite !W256.of_uintK !mod_R_W256_mod_R !R_mod_W256_R. by smt().
+rewrite /bool_of_uint256 /iszero in H0. by smt.
+
+seq 3 1: (
+#pre /\ denominator{1} = W256.of_int den{2} /\
+den{2} = (DOMAIN_SIZE * (at{2} - omegaPolyNum{2})) %% R
+).
+wp. skip. progress. 
+rewrite /addmod /mulmod. progress. rewrite !W256.of_uintK !R_mod_W256_R.
+have ->: DOMAIN_SIZE %% W256.modulus = DOMAIN_SIZE. by smt().
+have ->: (R - OMEGA ^ to_uint polyNum{1} %% R) %% W256.modulus = (R - OMEGA ^ to_uint polyNum{1} %% R). by smt().
+have ->: (to_uint at{1} + (R - OMEGA ^ to_uint polyNum{1} %% R)) %% R %% W256.modulus = (to_uint at{1} + (R - OMEGA ^ to_uint polyNum{1} %% R)) %% R. by smt().
+by smt().
+
+seq 1 1: (
+(polyNum{1}, at{1}) = (poly256, at256) /\
+(polyNum{2}, at{2}) = (to_uint poly256, to_uint at256) /\
+!Primops.reverted{1} /\
+omegaPower{1} = (of_int omegaPolyNum{2})%W256 /\
+omegaPolyNum{2} = OMEGA ^ polyNum{2} %% R /\
+tmp267{1} = (of_int atDomainSize{2})%W256 /\
+atDomainSize{2} = at{2} ^ DOMAIN_SIZE %% R /\
+ret{1} = (of_int num{2})%W256 /\
+num{2} = omegaPolyNum{2} * zd1{2} %% R /\
+zd1{2} = (atDomainSize{2} - 1) %% R /\ zd1{2} <> 0 /\
+denominator{1} = (of_int den{2})%W256 /\
+den{2} = DOMAIN_SIZE * (at{2} - omegaPolyNum{2}) %% R /\
+Primops.memory{1} = modexp_memory_footprint memory at{1} ((W256.of_int R) - (W256.of_int 2)) denominator{1} /\
+denominator{1} = W256.of_int inv{2} /\ inv{2} = (den{2} ^ (R - 2)) %% R
+).
+
+
+
+call (modexp_low_equiv_mid memory (W256.of_int OMEGA) poly256).
+skip. progress. by smt. by smt. 
+(* polyNum = 0 *)
+rcondf{1} 1. by progress.
+inline Modexp.mid. wp. skip. progress. by smt.
+have ->: polyNum{1} = W256.zero. by smt. progress. by smt.
+
+(* ((poly256 <> W256.zero /\ *)
+  (*   Primops.memory{1} = modexp_memory_footprint mem' at{1} (W256.of_int DOMAIN_SIZE) tmp267{1}) \/ *)
+  (*  (poly256 = W256.zero /\ *)
+  (*    Primops.memory{1} = modexp_memory_footprint memory at{1} (W256.of_int DOMAIN_SIZE) tmp267{1}) *)
+  (* ) *)
+
+seq 1 1 : (
+  (polyNum{1}, at{1}) = (poly256, at256) /\
+  (polyNum{2}, at{2}) = (to_uint poly256, to_uint at256) /\
+  !Primops.reverted{1} /\
+  omegaPower{1} = W256.of_int omegaPolyNum{2} /\
+  Primops.memory{1} = modexp_memory_footprint memory at{1} (W256.of_int DOMAIN_SIZE) tmp267{1} /\
+  tmp267{1} = W256.of_int atDomainSize{2}
+).
+
+exists* omegaPower{1}. elim* => oP.
+pose mem' := (modexp_memory_footprint memory ((of_int OMEGA))%W256 poly256 oP).
+case (poly256 = W256.zero).
+call (modexp_low_equiv_mid memory at256 (W256.of_int DOMAIN_SIZE)).
+skip. progress. by smt. by auto. 
+call (modexp_low_equiv_mid mem' at256 (W256.of_int DOMAIN_SIZE)).
+skip. progress. by smt. rewrite /mem'. case H0. progress. move => [? ?]. auto. apply modexp_same.
+
+seq 1 1: (#pre /\ ret{1} = W256.of_int zd1{2}). wp. skip. progress.
+rewrite /addmod. progress.
+rewrite !W256.of_uintK !R_mod_W256_R.  -(modzDm _ (-1) R) modNz. by smt(). by smt().
+simplify.
+
+    rewrite (modNz 1).
+
+
+
+have ->: (R - 1) %% W256.modulus = R - 1. by smt(). 
+have ->: (atDomainSize{2} %% W256.modulus + (R - 1)) = (atDomainSize{2} %% W256.modulus + (R - 1) %% W256.modulus). by smt().
+
+have : forall W256.of_int (a %% R)
+have ->: (atDomainSize{2} %% W256.modulus + (R - 1) %% W256.modulus) = (atDomainSize{2} + (R - 1)) %% W256.modulus.  
+
+    rcondf{1} 1. by progress.
 inline Modexp.mid. wp. skip. progress. rewrite /bool_of_uint256 in H0. by smt.
 
